Eliminate import opened
Don't `import opened` for `MessageHeader.Definitions` and `MessageHeaderValidity` (instead, I used the local names `Msg` and `V`, respectively).
This caused the need for some other imports that previously had been available via these opened imports.

src/SDK/MessageHeader/SerializeAAD.dfy
@@ -1,12 +1,13 @@
 include "Definitions.dfy"
 include "Validity.dfy"
+include "../Materials.dfy"
 
 include "../../Util/Streams.dfy"
 include "../../StandardLibrary/StandardLibrary.dfy"
 
 module MessageHeader.SerializeAAD {
-  import opened Definitions
-  import opened Validity
+  import V = Validity
+  import Materials
 
   import Streams
   import opened StandardLibrary
@@ -15,10 +16,10 @@ module MessageHeader.SerializeAAD {
   // ----- Specification -----
 
   function SerializeAAD(kvPairs: Materials.EncryptionContext): seq<uint8>
-    requires ValidAAD(kvPairs)
+    requires V.ValidAAD(kvPairs)
   {
-    reveal ValidAAD();
-    UInt16ToSeq(AADLength(kvPairs) as uint16) +
+    reveal V.ValidAAD();
+    UInt16ToSeq(V.AADLength(kvPairs) as uint16) +
     var n := |kvPairs|;
     if n == 0 then [] else
       UInt16ToSeq(n as uint16) +
@@ -26,27 +27,27 @@ module MessageHeader.SerializeAAD {
   }
 
   function SerializeKVPairs(kvPairs: Materials.EncryptionContext, lo: nat, hi: nat): seq<uint8>
-    requires forall i :: 0 <= i < |kvPairs| ==> ValidKVPair(kvPairs[i])
+    requires forall i :: 0 <= i < |kvPairs| ==> V.ValidKVPair(kvPairs[i])
     requires lo <= hi <= |kvPairs|
   {
     if lo == hi then [] else SerializeKVPairs(kvPairs, lo, hi - 1) + SerializeKVPair(kvPairs[hi - 1])
   }
 
   function SerializeKVPair(kvPair: (seq<uint8>, seq<uint8>)): seq<uint8>
-    requires ValidKVPair(kvPair)
+    requires V.ValidKVPair(kvPair)
   {
     UInt16ToSeq(|kvPair.0| as uint16) + kvPair.0 +
     UInt16ToSeq(|kvPair.1| as uint16) + kvPair.1
   }
 
-  // Function AADLength is defined without referring to SerializeAAD (because then
-  // these two would be mutually recursive with ValidAAD). The following lemma proves
+  // Function V.AADLength is defined without referring to SerializeAAD (because then
+  // these two would be mutually recursive with V.ValidAAD). The following lemma proves
   // that the two definitions correspond.
   lemma ADDLengthCorrect(kvPairs: Materials.EncryptionContext)
-    requires ValidAAD(kvPairs)
-    ensures |SerializeAAD(kvPairs)| == 2 + AADLength(kvPairs)
+    requires V.ValidAAD(kvPairs)
+    ensures |SerializeAAD(kvPairs)| == 2 + V.AADLength(kvPairs)
   {
-    reveal ValidAAD();
+    reveal V.ValidAAD();
     KVPairsLengthCorrect(kvPairs, 0, |kvPairs|);
     /**** Here's a more detailed proof:
     var n := |kvPairs|;
@@ -55,20 +56,20 @@ module MessageHeader.SerializeAAD {
       calc {
         |SerializeAAD(kvPairs)|;
       ==  // def. SerializeAAD
-        |UInt16ToSeq(AADLength(kvPairs) as uint16) + UInt16ToSeq(n as uint16) + s|;
+        |UInt16ToSeq(V.AADLength(kvPairs) as uint16) + UInt16ToSeq(n as uint16) + s|;
       ==  // UInt16ToSeq yields length-2 sequence
         2 + 2 + |s|;
       ==  { KVPairsLengthCorrect(kvPairs, 0, n); }
-        2 + 2 + KVPairsLength(kvPairs, 0, n);
+        2 + 2 + V.KVPairsLength(kvPairs, 0, n);
       }
     }
     ****/
   }
 
   lemma KVPairsLengthCorrect(kvPairs: Materials.EncryptionContext, lo: nat, hi: nat)
-    requires forall i :: 0 <= i < |kvPairs| ==> ValidKVPair(kvPairs[i])
+    requires forall i :: 0 <= i < |kvPairs| ==> V.ValidKVPair(kvPairs[i])
     requires lo <= hi <= |kvPairs|
-    ensures |SerializeKVPairs(kvPairs, lo, hi)| == KVPairsLength(kvPairs, lo, hi)
+    ensures |SerializeKVPairs(kvPairs, lo, hi)| == V.KVPairsLength(kvPairs, lo, hi)
   {
     /**** Here's a more detailed proof:
     if lo < hi {
@@ -80,14 +81,14 @@ module MessageHeader.SerializeAAD {
       ==
         |SerializeKVPairs(kvPairs, lo, hi - 1)| + |SerializeKVPair(kvPair)|;
       ==  { KVPairsLengthCorrect(kvPairs, lo, hi - 1); }
-        KVPairsLength(kvPairs, lo, hi - 1) + |SerializeKVPair(kvPair)|;
+        V.KVPairsLength(kvPairs, lo, hi - 1) + |SerializeKVPair(kvPair)|;
       ==  // def. SerializeKVPair
-        KVPairsLength(kvPairs, lo, hi - 1) +
+        V.KVPairsLength(kvPairs, lo, hi - 1) +
         |UInt16ToSeq(|kvPair.0| as uint16) + kvPair.0 + UInt16ToSeq(|kvPair.1| as uint16) + kvPair.1|;
       ==
-        KVPairsLength(kvPairs, lo, hi - 1) + 2 + |kvPair.0| + 2 + |kvPair.1|;
-      ==  // def. KVPairsLength
-        KVPairsLength(kvPairs, lo, hi);
+        V.KVPairsLength(kvPairs, lo, hi - 1) + 2 + |kvPair.0| + 2 + |kvPair.1|;
+      ==  // def. V.KVPairsLength
+        V.KVPairsLength(kvPairs, lo, hi);
       }
     }
     ****/
@@ -96,9 +97,9 @@ module MessageHeader.SerializeAAD {
   // ----- Implementation -----
 
   method SerializeAADImpl(os: Streams.StringWriter, kvPairs: Materials.EncryptionContext) returns (ret: Result<nat>)
-    requires os.Valid() && ValidAAD(kvPairs)
+    requires os.Valid() && V.ValidAAD(kvPairs)
     modifies os`data
-    ensures os.Valid() && ValidAAD(kvPairs)
+    ensures os.Valid() && V.ValidAAD(kvPairs)
     ensures match ret
       case Success(totalWritten) =>
         var serAAD := SerializeAAD(kvPairs);
@@ -108,7 +109,7 @@ module MessageHeader.SerializeAAD {
         && os.data == old(os.data) + serAAD
       case Failure(e) => true
   {
-    reveal ValidAAD();
+    reveal V.ValidAAD();
     var totalWritten := 0;
 
     // Key Value Pairs Length (number of bytes of total AAD)
@@ -159,10 +160,10 @@ module MessageHeader.SerializeAAD {
 
   method ComputeAADLength(kvPairs: Materials.EncryptionContext) returns (res: Result<uint16>)
     requires |kvPairs| < UINT16_LIMIT
-    requires forall i :: 0 <= i < |kvPairs| ==> ValidKVPair(kvPairs[i])
+    requires forall i :: 0 <= i < |kvPairs| ==> V.ValidKVPair(kvPairs[i])
     ensures match res
-      case Success(len) => len as int == AADLength(kvPairs)
-      case Failure(_) => UINT16_LIMIT <= AADLength(kvPairs)
+      case Success(len) => len as int == V.AADLength(kvPairs)
+      case Failure(_) => UINT16_LIMIT <= V.AADLength(kvPairs)
   {
     var n: int32 := |kvPairs| as int32;
     if n == 0 {
@@ -172,11 +173,11 @@ module MessageHeader.SerializeAAD {
       var i: int32 := 0;
       while i < n
         invariant i <= n
-        invariant 2 + KVPairsLength(kvPairs, 0, i as int) == len as int < UINT16_LIMIT
+        invariant 2 + V.KVPairsLength(kvPairs, 0, i as int) == len as int < UINT16_LIMIT
       {
         var kvPair := kvPairs[i];
         len := len + 4 + |kvPair.0| as int32 + |kvPair.1| as int32;
-        KVPairsLengthSplit(kvPairs, 0, i as int + 1, n as int);
+        V.KVPairsLengthSplit(kvPairs, 0, i as int + 1, n as int);
         if limit <= len {
           return Failure("The number of bytes in encryption context exceeds the allowed maximum");
         }
